src/Util/VectorUtil.v
@@ -1,36 +1,137 @@
 Set Warnings "-local-declaration,-scope".
 
-From Coq Require Import Equality Vector.
+From Coq Require Import Basics Bool Equality ProofIrrelevance Vector.
 Import VectorNotations.
 
 (* Deconstruct a non-empty vector. *)
 Definition Vector_uncons {A} {n : nat} (v : Vector.t A (S n)) :
-  A * Vector.t A n :=
-  match v in Vector.t _ Sn
-        return match Sn with
-               | O => unit (* unreachable *)
-               | S n => _
-               end
-  with
-  | [] => tt
-  | x :: xs => (x, xs)
-  end.
+  A * Vector.t A n := (hd v, tl v).
 
 Fixpoint splitAt {A} (l : nat) {r : nat} :
   Vector.t A (l + r) -> Vector.t A l * Vector.t A r :=
   match l with
   | 0 => fun v => ([], v)
   | S l' => fun v =>
-    let (b, v') := Vector_uncons v in
-    let (v1, v2) := splitAt l' v' in
-    (b::v1, v2)
+    let (v1, v2) := splitAt l' (tl v) in
+    (hd v::v1, v2)
   end.
 
 Theorem split_append {A} (l : nat) : forall {r : nat} (v : Vector.t A l) (w : Vector.t A r),
     splitAt l (append v w) = (v, w).
 Proof with simpl; auto.
-  induction l; intros...
-  - dependent destruction v...
-  - dependent destruction v...
-    rewrite IHl...
+  induction l; intros; dependent destruction v...
+  rewrite IHl...
+Qed.
+
+Open Scope program_scope.
+Open Scope bool_scope.
+
+Definition forallb {A n} (f : A -> bool) : Vector.t A n -> bool :=
+  fold_left (fun x => andb x ∘ f) true.
+
+Definition existsb {A n} (f : A -> bool) : Vector.t A n -> bool :=
+  fold_left (fun x => orb x ∘ f) false.
+
+Lemma fold_left_id {A B n} (f : B -> A -> B) (base : B) :
+  (forall a : A, f base a = base) ->
+  forall v : Vector.t A n,
+    fold_left f base v = base.
+Proof with simpl; auto.
+  induction v...
+  rewrite H...
+Qed.
+
+Corollary forallb_cons {A n} (f : A -> bool) (a : A) (v : Vector.t A n) :
+  forallb f (a::v) = f a && forallb f v.
+Proof with simpl; auto.
+  intros.
+  unfold forallb.
+  unfold compose...
+  destruct (f a)...
+  apply fold_left_id...
+Qed.
+
+Corollary existsb_cons {A n} (f : A -> bool) (a : A) (v : Vector.t A n) :
+  existsb f (a::v) = f a || existsb f v.
+Proof with simpl; auto.
+  intros.
+  unfold existsb.
+  unfold compose...
+  destruct (f a)...
+  apply fold_left_id...
+Qed.
+
+Theorem forallb_true_iff {A n} (f : A -> bool) :
+  forall (v : Vector.t A n),
+    forallb f v = true <-> Forall (eq true ∘ f) v.
+Proof with unfold compose in *; simpl in *; auto.
+  induction v; split; intros...
+  - constructor.
+  - rewrite forallb_cons in H.
+    apply andb_prop in H.
+    destruct H.
+    constructor...
+    apply IHv...
+  - rewrite forallb_cons.
+    apply andb_true_iff.
+    inversion H; subst...
+    apply inj_pair2 in H2; subst...
+    split...
+    apply IHv...
+Qed.
+
+Theorem existsb_true_iff {A n} (f : A -> bool) :
+  forall (v : Vector.t A n),
+    existsb f v = true <-> Exists (eq true ∘ f) v.
+Proof with unfold compose in *; simpl in *; auto.
+  induction v; split; intros...
+  - inversion H.
+  - inversion H.
+  - rewrite existsb_cons in H.
+    apply orb_true_iff in H.
+    destruct H...
+    + apply Exists_cons_hd...
+    + apply Exists_cons_tl...
+      apply IHv...
+  - rewrite existsb_cons.
+    apply orb_true_iff.
+    inversion H; subst...
+    apply inj_pair2 in H3; subst...
+    right.
+    apply IHv...
+Qed.
+
+Theorem forall_exists {A n} (f : A -> bool) :
+  forall v : Vector.t A n,
+    forallb f v = negb (existsb (negb ∘ f) v).
+Proof with simpl; auto.
+  induction v...
+  unfold forallb.
+  unfold existsb.
+  unfold compose...
+  destruct (f h)...
+  repeat rewrite fold_left_id...
+Qed.
+
+Lemma fold_left_eq {A B} {n : nat} (f1 f2 : B -> A -> B) :
+  (forall b a, f1 b a = f2 b a) ->
+  forall (v : Vector.t A n) (b : B), fold_left f1 b v = fold_left f2 b v.
+Proof with simpl; auto.
+  intro.
+  induction v...
+  intro.
+  rewrite H...
+Qed.
+
+Theorem exists_forall {A n} (f : A -> bool)
+  (v : Vector.t A n) :
+    existsb f v = negb (forallb (negb ∘ f) v).
+Proof with simpl; auto.
+  rewrite forall_exists.
+  unfold existsb.
+  unfold compose.
+  rewrite negb_involutive.
+  eapply fold_left_eq.
+  intros.
+  rewrite negb_involutive...
 Qed.
